Veir/Dialects/ModArith/ModArith.lean
@@ -29,11 +29,42 @@ theorem BarretReduceSpecImpliesLt2q (m x r : Nat) :
     have hlt := Nat.mod_lt x hBounds.left
     grind
 
-theorem barrettReduceStepNatCorrect (m x : Nat) :
-  ∀ output, barrettReduceStepNat m x = output  →
+-- theorem AssumingQ (m x r : Nat) :
+--   ∀ m x:
+--   let bitWidth := natBitLength (m - 1)
+--   let k := 2 * bitWidth
+--   let mu := ((1 : Nat) <<< k) / m
+--   let q := (a * mu) >>> k
+--   BarretPrecondition m x → ((q = x / m) ∨ (q = x/m)) := by
+--   sorry
+
+theorem barrettReduceStepNatCorrect (m x output : Nat) :
+    barrettReduceStepNat m x = output  →
     BarrettReduceSpec m x output := by
-    intro output hOutput
+    intro h
     simp [BarrettReduceSpec, BarretPrecondition]
     intro h0 hmm
-    unfold barrettReduceStepNat at hOutput
+    unfold barrettReduceStepNat at h
+    /- We need to show that the weird shift division hack is the same. -/
+    /- lets focus first on the precomputed constant, mu? -/
+    /- we have mu = 2^(2w) / m which is what?  -/
+    /- if m = 222 and bw=8, then we have 2^16/222 = 65k/222 = 295.something ??-/
+    /- Now we take x*295 and shift down by 2w? -/
+    /- effectively, we divide by 2^2w = 2^16 again?-/
+    /- lets say x = 333 --> 98235/2^15 i.e. 65536 gives 1.49 for q?-/
+    /- now we compute x - 1 * m and oh boy, it worked! -/
+    /- so when do we end up in +m range? -/
+    /- basically, in the nice case, q is exactly x/m floordiv? -/
+    /- and in the not so nice case, x/m floordiv + 1 ? -/
+    /- Basically, we look at 2^(log2(m)/m) basically,  -/
     sorry
+
+theorem barretReduceFullCorrect (m x : Nat) :
+∀ output : Nat, ∀ y : Nat,
+  (BarretPrecondition m x ∧ barrettReduceStepNat m x = y ∧ subifgeNat m y = output) →
+  output = x % m := by
+  intro output y h
+  have hPre := h.left
+  have hStep := h.right.left
+  have hSubIfge := h.right.right
+  sorry
